hfc/FFAMemoryHypCallTestingInterface.v
@@ -48,6 +48,7 @@ Local Open Scope string_scope.
 Require Import Coqlib sflib.
 
 (* From HafniumCore *)
+Require Import Any.
 Require Import Lang.
 Require Import Values.
 Require Import Integers.
@@ -200,48 +201,36 @@ Notation " 'check' A ;;; B" :=
  
 Local Open Scope itree_monad_scope.
 
+
+
 (***********************************************************************)
-(** *                 Context switching related parts                  *)
+(** *                 Instantiations for contexts                      *)
 (***********************************************************************)
+(** We provides instantiations for the context that our specifiction
+    relies on. *)
+
+(***********************************************************************)
+(** **            FFA_TYPES_AND_CONSTANTS instance                     *)
+(***********************************************************************)
+Definition ffa_memory_region_tag_t := Z.
+Definition granuale_shift := 12.
 
 Global Instance ffa_types_and_constants : FFA_TYPES_AND_CONSTANTS :=
   {
-  ffa_memory_region_tag_t := Z;
+  ffa_memory_region_tag_t := ffa_memory_region_tag_t;
   (** - The following two types are for message passings. We use them to record and 
         retrieve descriptor information *)
-  ffa_mailbox_send_msg_t := Z;
-  ffa_mailbox_recv_msg_t := Z;
 
   (** - Granuale value. It is usually a multiplication of 4096 (4KiB) *)
-  granuale := 4096;
+  granuale := Z.shiftl 1 granuale_shift;
   init_ffa_memory_region_tag := 0;
-  init_ffa_mailbox_send_msg  := 0;
-  init_ffa_mailbox_recv_msg  := 0;  
   }.
 
-Global Instance address_translation
-  : AddressTranslation (ffa_types_and_constants := ffa_types_and_constants) :=
-  {
-  hafnium_address_translation_table := fun x => Some x;
-  vm_address_translation_table := fun vid x => Some x;
-  }.
-
-Global Instance  hafnium_memory_management_context
-  : HafniumMemoryManagementContext (address_translation := address_translation) :=
-  {
-  address_low := 0;
-  address_high := Z.pow 2 16;
-  alignment_value := granuale;
-  }.
-
-Global Instance vm_context
-  : VMContext (ffa_types_and_constants := ffa_types_and_constants) :=
-  {
-  vcpu_max_num := 8
-  }.
-  
-Global Instance  handle_context :
-  HandleContext (ffa_types_and_constants := ffa_types_and_constants) :=
+(***********************************************************************)
+(** **                  DescriptorContext instance                     *)
+(***********************************************************************)
+Global Instance descriptor_context :
+  DescriptorContext (ffa_types_and_constants := ffa_types_and_constants) :=
   {
   make_handle := fun vid value =>
                    if decide (0 <= vid < (Z.shiftl 1 16))
@@ -256,81 +245,310 @@ Global Instance  handle_context :
                   Z.shiftr handle 16;
   }.
 
-Print ZTree.empty.
 
+(***********************************************************************)
+(** **                  FFA_VM_CONTEXT instance                        *)
+(***********************************************************************)
+Inductive ffa_mailbox_msg_t : Type :=
+| mailbox_memory_init_value
+| mailbox_memory_region (region_descriptor: FFA_memory_region_struct)
+| mailbox_memory_relinquish (relinquish_descriptor: FFA_memory_relinquish_struct)
+| mailbox_z (value : Z).
+
+Definition init_ffa_mailbox_msg := mailbox_memory_init_value.
+Definition vcpu_max_num := 4.
+
+Definition mailbox_msg_to_region_struct :=
+  fun x =>
+    match x with
+    | mailbox_memory_region region_descriptor =>
+      Some region_descriptor
+    | _ => None
+    end.
+
+Definition mailbox_msg_to_relinquish_struct :=
+  fun x =>
+    match x with
+    | mailbox_memory_relinquish relinquish_descriptor =>
+      Some relinquish_descriptor
+    | _ => None
+    end.
+
+Definition mailbox_msg_to_z :=
+  fun x =>
+    match x with
+    | mailbox_z value =>
+      Some value
+    | _ => None
+    end.
+
+Definition region_struct_to_mailbox_msg :=
+  fun x => Some (mailbox_memory_region x).
+
+Definition relinquish_struct_to_mailbox_msg :=
+  fun x => Some (mailbox_memory_relinquish x).
+
+Definition z_to_mailbox_msg := 
+  fun x => Some (mailbox_z x).
+
+Global Instance ffa_vm_context :
+  FFA_VM_CONTEXT (ffa_types_and_constants := ffa_types_and_constants)  :=
+    {
+    (** - The following two types are for message passings. We use them to record and 
+        retrieve descriptor information *)
+    ffa_mailbox_send_msg_t := ffa_mailbox_msg_t;
+    ffa_mailbox_recv_msg_t := ffa_mailbox_msg_t;
+    init_ffa_mailbox_send_msg := init_ffa_mailbox_msg;
+    init_ffa_mailbox_recv_msg := init_ffa_mailbox_msg;
+
+    vcpu_max_num := vcpu_max_num;
+
+    (** mailbox to/from descriptors *)
+    mailbox_send_msg_to_region_struct := mailbox_msg_to_region_struct;
+    mailbox_send_msg_to_relinqiush_struct := mailbox_msg_to_relinquish_struct;
+    mailbox_send_msg_to_Z := mailbox_msg_to_z;
+    region_struct_to_mailbox_send_msg := region_struct_to_mailbox_msg;
+    relinqiush_struct_to_mailbox_send_msg := relinquish_struct_to_mailbox_msg;
+    Z_to_mailbox_send_msg := z_to_mailbox_msg;
+
+    mailbox_recv_msg_to_region_struct := mailbox_msg_to_region_struct;
+    mailbox_recv_msg_to_relinqiush_struct := mailbox_msg_to_relinquish_struct;
+    mailbox_recv_msg_to_Z := mailbox_msg_to_z;
+    region_struct_to_mailbox_recv_msg := region_struct_to_mailbox_msg;
+    relinqiush_struct_to_mailbox_recv_msg := relinquish_struct_to_mailbox_msg;
+    Z_to_mailbox_recv_msg := z_to_mailbox_msg;
+
+    primary_vm_id := 1;
+    secondary_vm_ids := 2::3::4::nil;
+
+    (* TODO: Need to fix *)
+    FFA_memory_region_struct_size := fun x => 36;
+    }.
+    
+(** TODO: The following values are dummy representations. We have to provide 
+    proper values later if we want to connect this one with the real Hafnium / other 
+    hypervisor implementations *)
+
+(***********************************************************************)
+(** **       HafniumMemoryManagementContext instance                   *)
+(***********************************************************************)
+
+Definition address_low_shift := 30.
+Definition address_high_shift := 32.
+
+Global Instance hafnium_memory_management_basic_context
+  : HafniumMemoryManagementBasicContext
+      (ffa_vm_context := ffa_vm_context) :=
+  {
+  address_low := (Z.shiftl 1 address_low_shift)%Z;
+  address_high := (Z.shiftl 1 address_high_shift - 1)%Z;
+  alignment_value := granuale; (* 4096 *)
+  }.
+
+Definition hafnium_address_translation_table :=
+  fun (x : ffa_address_t) =>
+    if decide (address_low <= x)%Z && decide (x < address_high)%Z
+    then Some x else None.
+
+Definition vm_address_translation_table :=
+  fun (vid : ffa_UUID_t) (x : ffa_address_t) =>
+    if decide (0 <= vid)%Z && decide (vid < number_of_vm)%Z
+    then if decide (address_low <= x)%Z && decide (x < address_high)%Z
+         then Some x
+         else None
+    else None.  
+
+Global Instance hafnium_memory_management_context
+  : HafniumMemoryManagementContext
+      (hafnium_memory_management_basic_context
+         := hafnium_memory_management_basic_context) :=
+  {
+  hafnium_address_translation_table :=
+    hafnium_address_translation_table;
+  vm_address_translation_table :=
+    vm_address_translation_table;
+  }.
+
+(***********************************************************************)
+(** **                 AbstractStateContext instance                   *)
+(***********************************************************************)
+
+Definition init_cpu_id := 0.
+Definition num_of_cpus := 8.
+
+Definition init_CPU_struct := mkCPU_struct.
+
+Fixpoint cal_init_cpus (cpu_nums : nat) :=
+  match cpu_nums with
+  | O =>  (ZTree.empty CPU_struct)
+  | S n' =>
+    let res :=  cal_init_cpus n' in
+    ZTree.set (Z.of_nat cpu_nums) 
+              init_CPU_struct res
+  end.
+
+Definition init_cpus := cal_init_cpus (Z.to_nat num_of_cpus).
+
+Definition init_api_page_pool_size_shift := 14.
+
+Definition init_mem_global_properties :=
+  mkMemGlobalProperties
+    NotOwned NoAccess 
+    FFA_INSTRUCTION_ACCESS_NOT_SPECIFIED
+    FFA_DATA_ACCESS_NOT_SPECIFIED
+    FFA_MEMORY_NOT_SPECIFIED_MEM
+    MemClean.
+    
+Fixpoint cal_init_global_properties_pool
+         (address : nat)  :=
+  match address with 
+  | O => if decide (0 >= address_low)
+        then ZTree.set (Z.shiftl 0 granuale_shift)  
+                       init_mem_global_properties
+                       (ZTree.empty MemGlobalProperties)
+        else (ZTree.empty MemGlobalProperties)
+  | S n' =>
+    let converted_addr := Z.shiftl (Z.of_nat address) granuale_shift in
+    if decide (converted_addr >= address_low)
+    then let res := cal_init_global_properties_pool n' in
+         ZTree.set converted_addr  
+                   init_mem_global_properties
+                   res
+    else (ZTree.empty MemGlobalProperties)
+  end.         
+  
 Definition init_mem_global_properties_pool
   : mem_global_properties_pool
-  := ZTree.empty MemGlobalProperties.
+  := cal_init_global_properties_pool
+       (Z.to_nat (Z.shiftr address_high granuale_shift)).
+
+Fixpoint cal_init_local_properties_pool
+         (vms : list Z) :=
+  match vms with 
+  | nil => (ZTree.empty
+             (ZTree.t MemLocalProperties))
+  | hd::tl =>
+    let res := cal_init_local_properties_pool tl in
+    ZTree.set hd (ZTree.empty MemLocalProperties) res
+  end.         
 
 Definition init_mem_local_properties_global_pool 
   : mem_local_properties_global_pool
-  := ZTree.empty
-       (ZTree.t MemLocalProperties).
+  :=  cal_init_local_properties_pool vm_ids.
 
 Definition init_mem_properties :=
   mkMemProperties
     init_mem_global_properties_pool
     init_mem_local_properties_global_pool.
 
+Definition init_VM_COMMON_struct (vcpu_ids: list Z) 
+  := mkVM_COMMON_struct
+       None
+       vcpu_ids 
+       (ZTree.empty VCPU_struct).
+
+Definition init_MAILBOX_struct :=
+  mkMAILBOX_struct
+    init_ffa_mailbox_msg
+    init_ffa_mailbox_msg
+    None (* recv_sender *)
+    0 (* recv_size *)
+    None (* recv func *)
+.
+
+Definition init_VM_KERNEL_context (vcpu_ids: list Z) :=
+ mkVM_KERNEL_struct 
+   (init_VM_COMMON_struct vcpu_ids)
+   init_MAILBOX_struct.
+
+Fixpoint cal_init_VM_KERNEL_contexts (vm_ids: list Z) := 
+  match vm_ids with
+  | nil =>  (ZTree.empty VM_KERNEL_struct)
+  | hd::tl =>
+    let res :=  cal_init_VM_KERNEL_contexts tl in
+    ZTree.set hd (init_VM_KERNEL_context (hd::nil)) res
+  end.
+
+Definition init_VM_KERNEL_contexts :=
+  cal_init_VM_KERNEL_contexts vm_ids.
+
+Fixpoint cal_init_VM_USERSPACE_contexts (vm_ids: list Z) :=
+  match vm_ids with
+  | nil =>  (ZTree.empty VM_USERSPACE_struct)
+  | hd::tl =>
+    let res :=  cal_init_VM_USERSPACE_contexts tl in
+    ZTree.set hd (mkVM_USERSPACE_struct (init_VM_COMMON_struct (hd::nil))) res
+  end.
+
+Definition init_VM_USERSPACE_contexts :=
+  cal_init_VM_USERSPACE_contexts vm_ids.
+
 Definition init_hypervisor_struct :=
   mkHypervisor_struct
-    0 8 (ZTree.empty CPU_struct)
-    false None
-    4096
-    (ZTree.empty FFA_memory_share_state_struct)
-    0
-    init_mem_properties
-    0
-    (ZTree.empty VM_struct).
+    init_cpu_id
+    num_of_cpus
+    init_cpus
+    false (* time slice enabled *)
+    None (* tpidr_el2 *)
+    (Z.shiftl 1 init_api_page_pool_size_shift) (* api_page_pool_size *)
+    (ZTree.empty FFA_memory_share_state_struct) (* ffa_share_state *)
+    0 (* fresh_index_for_ffa_share_state *)
+    init_mem_properties (* mem_properties *)
+    number_of_vm  (* vm_count *)
+    init_VM_KERNEL_contexts.
 
-Definition init_vms_userspaces := ZTree.empty VM_USERSPACE_struct.
+(* TODO: it is a dummy value *)
+Definition version_number := (1, 1).
 
 Definition init_abstract_state :=
-  mkAbstractState (1, 1) 1 init_hypervisor_struct init_vms_userspaces.
+  mkAbstractState
+    (1, 1) (* dummy version number *)
+    1 (*  cur_entity_id - primary VM *)
+    init_hypervisor_struct
+    init_VM_USERSPACE_contexts.
+
+Fixpoint find_next_entity (vm_ids : list ffa_UUID_t)
+         (current_entity_id : ffa_UUID_t) :=
+  match vm_ids with
+  | nil => primary_vm_id
+  | hd::tl =>
+    if decide (current_entity_id = hd)
+    then match tl with
+         | nil => primary_vm_id
+         | hd'::_ => hd'
+         end
+    else find_next_entity tl current_entity_id
+  end.
+
+Definition scheduler (st: AbstractState) : ffa_UUID_t :=
+  let cur_entity_id := st.(cur_entity_id) in
+  find_next_entity vm_ids cur_entity_id.  
 
 Global Instance abstract_state_context :
   AbstractStateContext
     (ffa_types_and_constants := ffa_types_and_constants)
-    (address_translation := address_translation)
-    (hafnium_memory_management_context := hafnium_memory_management_context) 
-    (vm_context := vm_context)
-    (handle_context := handle_context) :=
+    (descriptor_context := descriptor_context)
+    (ffa_vm_context := ffa_vm_context)
+    (hafnium_memory_management_basic_context
+       := hafnium_memory_management_basic_context)
+    (hafnium_memory_management_context
+       := hafnium_memory_management_context) :=
   {
-  primary_vm_id := 1;
-  secondary_vm_ids := 2::3::4::5::6::7::nil;
-    
-  mailbox_send_msg_to_region_struct :=
-    fun x => Some init_FFA_memory_region_struct;
-  mailbox_send_msg_to_relinqiush_struct :=
-    fun x => Some init_FFA_mem_relinquish_struct;
-  mailbox_send_msg_to_Z :=
-    fun x => Some 0;
-  region_struct_to_mailbox_send_msg :=
-    fun x => Some 0;    
-  relinqiush_struct_to_mailbox_send_msg :=
-    fun x => Some 0;
-  Z_to_mailbox_send_msg := 
-    fun x => Some 0;
-
-  mailbox_recv_msg_to_region_struct :=
-    fun x => Some init_FFA_memory_region_struct;
-  mailbox_recv_msg_to_relinqiush_struct :=
-    fun x => Some init_FFA_mem_relinquish_struct;
-  mailbox_recv_msg_to_Z :=
-    fun x => Some 0;
-  region_struct_to_mailbox_recv_msg :=
-    fun x => Some 0;
-  relinqiush_struct_to_mailbox_recv_msg :=
-    fun x => Some 0;
-  Z_to_mailbox_recv_msg := 
-    fun x => Some 0;
-
-  scheduler :=
-    fun x => 0;
-
-  FFA_memory_region_struct_size := fun x => 36;
-  initial_state := init_abstract_state   
+      scheduler := scheduler;
+      initial_state := init_abstract_state;
   }.
+
+
+
+Instance abstract_state_Showable: Showable AbstractState :=
+  {
+  show :=
+    fun x => " "
+  }.
+
+(***********************************************************************)
+(** *                 Context switching related parts                  *)
+(***********************************************************************)
 
 Section FFAContextSwitching.
 
@@ -375,21 +593,29 @@ Section FFAContextSwitching.
     itree HypervisorEE (unit) := 
     st <- trigger GetState;;
     (* check whether the current running entity is one of VMs *)
-    if decide (st.(cur_entity_id) <> hafnium_id) && in_dec zeq st.(cur_entity_id) vm_ids
+    if decide (st.(cur_entity_id) <> hafnium_id) &&
+       in_dec zeq st.(cur_entity_id) vm_ids
     then (* get contexts for the currently running entity ID *)
       do vm_userspace <- ZTree.get st.(cur_entity_id) st.(vms_userspaces) ;;;
-      do vcpu_regs <- ZTree.get vm_userspace.(userspace_cur_vcpu_index) vm_userspace.(userspace_vcpus) ;;;
+      do cur_vcpu_index <- (vm_userspace.(vm_userspace_context).(cur_vcpu_index)) ;;;
+      do vcpu_regs <- ZTree.get cur_vcpu_index 
+                       (vm_userspace.(vm_userspace_context).(vcpus_contexts)) ;;;
+                                                                         
       (* get vm contexts in Hanfium to save the userspace information in it *)              
       do vm_context <- ZTree.get st.(cur_entity_id) st.(hypervisor_context).(vms_contexts) ;;;
-      if decide (vm_context.(vcpu_num) = vm_userspace.(userspace_vcpu_num)) &&
+      if decide (list_eq_dec zeq (vm_context.(vm_kernelspace_context).(vcpus)) 
+                             (vm_userspace.(vm_userspace_context).(vcpus))) &&
          decide (vcpu_regs.(vm_id) = Some st.(cur_entity_id))
       then
-        let new_vcpu_id := vm_userspace.(userspace_cur_vcpu_index) in
-        let new_vm_context := vm_context {vm_cur_vcpu_index: new_vcpu_id}
-                                         {vm_vcpus:
-                                            ZTree.set new_vcpu_id vcpu_regs vm_context.(vcpus)} in
+        let new_vm_context :=
+            vm_context {vm_cur_vcpu_index: Some cur_vcpu_index}
+                       {vm_vcpus_contexts:
+                          ZTree.set cur_vcpu_index vcpu_regs
+                                    vm_context.(vm_kernelspace_context).(vcpus_contexts)} in
         let new_vms_contexts :=
-            ZTree.set st.(cur_entity_id) new_vm_context st.(hypervisor_context).(vms_contexts) in
+            ZTree.set st.(cur_entity_id)
+                           new_vm_context
+                           st.(hypervisor_context).(vms_contexts) in
         let new_st := st {cur_entity_id: hafnium_id}
                          {hypervisor_context/tpidr_el2: Some vcpu_regs}
                          {hypervisor_context/vms_contexts: new_vms_contexts} in 
@@ -420,16 +646,22 @@ Section FFAContextSwitching.
       (** get vm context to restore the userspace information *)
       do vm_context <- ZTree.get next_vm_id st.(hypervisor_context).(vms_contexts) ;;;
       (** get vcpu register information *)
-      do vcpu_regs <- ZTree.get vm_context.(cur_vcpu_index) vm_context.(vcpus) ;;;
-         if decide (vm_context.(vcpu_num) = vm_userspace.(userspace_vcpu_num)) &&
-            decide (vm_context.(cur_vcpu_index) = vm_userspace.(userspace_cur_vcpu_index)) &&
+      do cur_kernel_vcpu_index <- (vm_context.(vm_kernelspace_context).(cur_vcpu_index)) ;;;
+      do cur_user_vcpu_index <- (vm_userspace.(vm_userspace_context).(cur_vcpu_index)) ;;;
+      do vcpu_regs <- ZTree.get cur_kernel_vcpu_index
+                               (vm_context.(vm_kernelspace_context).(vcpus_contexts)) ;;;
+         if decide (list_eq_dec zeq (vm_context.(vm_kernelspace_context).(vcpus))
+                                vm_userspace.(vm_userspace_context).(vcpus)) &&
+            decide (cur_kernel_vcpu_index = cur_user_vcpu_index) &&
             decide (vcpu_regs.(vm_id) = Some next_vm_id)
             (* TODO: add cpu connection check with vcpu_regs later *)
          then
            let new_vm_userspace := 
-               vm_userspace {userspace_vcpus :
-                               (ZTree.set (vm_userspace.(userspace_cur_vcpu_index))
-                                          vcpu_regs (vm_userspace.(userspace_vcpus)))} in
+               vm_userspace
+                 {client_vcpus_contexts :
+                    (ZTree.set cur_kernel_vcpu_index
+                               vcpu_regs
+                               (vm_userspace.(vm_userspace_context).(vcpus_contexts)))} in
            let new_vms_userspaces :=
                ZTree.set next_vm_id new_vm_userspace st.(vms_userspaces) in
            let new_st := st {cur_entity_id: next_vm_id}
@@ -504,17 +736,21 @@ Section FFADispatch.
                  ZTree.get
                    vid
                    updated_st.(hypervisor_context).(vms_contexts);;;
+              do cur_kernel_vcpu_index <-
+                 vm_context.(vm_kernelspace_context).(cur_vcpu_index) ;;;
               do vcpu_reg <-
-                 ZTree.get
-                   vm_context.(cur_vcpu_index) vm_context.(vcpus);;;
+                 ZTree.get cur_kernel_vcpu_index 
+                    vm_context.(vm_kernelspace_context).(vcpus_contexts);;;
               let new_vcpu_reg :=
                   mkVCPU_struct (vcpu_reg.(cpu_id)) (vcpu_reg.(vm_id))
                                 (mkArchRegs (ffa_value_gen ffa_result)) in
               let new_vm_context := 
                   vm_context
-                    {vm_vcpus: ZTree.set (vm_context.(cur_vcpu_index))
-                                         new_vcpu_reg 
-                                         vm_context.(vcpus)} in
+                    {vm_vcpus_contexts:
+                       ZTree.set
+                         cur_kernel_vcpu_index
+                         new_vcpu_reg 
+                         vm_context.(vm_kernelspace_context).(vcpus_contexts)} in
               let new_st :=
                   updated_st
                     {hypervisor_context / vms_contexts:
